scratch: self app arm

scratch/FuelInflationCounterexample.v
@@ -1,5 +1,5 @@
 From SymCoreTheory Require Import SymCore ConCore Completeness Model.
-From Stdlib Require Import Strings.String Lists.List Bool.Bool Arith.PeanoNat Lia.
+From Stdlib Require Import Strings.String Lists.List Bool.Bool Arith.PeanoNat Arith.Wf_nat Lia.
 Import ListNotations.
 Open Scope string_scope.
 
@@ -15,7 +15,7 @@ Fixpoint nots (e : expr) : nat :=
   | _ => O
   end.
 
-Definition inflation (j : expr) : nat := 10 + 3 * nots j.
+Definition inflation (j : expr) : nat := 10 + 5 * nots j.
 
 Fixpoint inflate_not (a : expr) : expr :=
   match a with
@@ -226,4 +226,199 @@ Proof.
     fuel_reduce_prim_contains fuel_reduce_prim_denote fuel_reduce_prim_ground_value
     fuel_reduce_prim_ite_contains model_cast_expr_contains
     model_subst_coerc_contains_env model_subst_type_contains_env).
+Qed.
+
+Inductive tower : expr -> Prop :=
+  | Tower_Bot : tower (EBot BOutOfFuel)
+  | Tower_Not : forall a, tower a -> tower (EApp (EPrimOp PNot) a).
+
+Lemma tower_flat_ground : forall a, tower a -> flat a = true /\ smt_ground a = false.
+Proof.
+  intros a H. induction H as [| a _ [Hf Hg]]; [split; reflexivity |].
+  simpl. rewrite Hf, Hg. split; reflexivity.
+Qed.
+
+Lemma reduce_not_tower : forall a,
+  tower a -> reduce_prim PNot (a :: nil) = EApp (EPrimOp PNot) a.
+Proof.
+  intros a H. destruct (tower_flat_ground a H) as [Hf Hg].
+  assert (Hp : inflate_not a = model_reduce_prim PNot (a :: nil))
+    by (destruct H; reflexivity).
+  cbn [reduce_prim fuel_solver fuel_reduce_prim]. rewrite Hp.
+  unfold model_reduce_prim, op_spine. cbn [length model_arity Nat.eqb fold_left].
+  rewrite lift_flat by (simpl; rewrite Hf; reflexivity).
+  simpl. unfold fold_leaf. simpl. rewrite Hg. reflexivity.
+Qed.
+
+Definition gv : var := "g".
+Definition junk_arg : expr := EApp (EVar gv) (EVar gv).
+Definition junk_body : expr := EApp (EPrimOp PNot) junk_arg.
+Definition junk_fun : expr := ELam gv junk_body.
+Definition junk : expr := EApp junk_fun junk_fun.
+
+Inductive resolves : nat -> environment -> Prop :=
+  | Resolves_Fun : forall Γ Γ0,
+      lookup_env Γ gv = Some (Γ0, junk_fun) -> resolves 0 Γ
+  | Resolves_Link : forall i Γ Γ0,
+      lookup_env Γ gv = Some (Γ0, EVar gv) -> resolves i Γ0 -> resolves (S i) Γ.
+
+Ltac kill_rule :=
+  match goal with
+  | [ Hs : sat _ = false |- _ ] => discriminate Hs
+  | [ Hu : unspool_app _ _ = (ECon _, _) |- _ ] => discriminate Hu
+  | [ Hu : unspool_app _ _ = (EIf _ _ _, _) |- _ ] => discriminate Hu
+  | [ Hu : unspool_app _ _ = (EPrimOp _, _) |- _ ] => discriminate Hu
+  | [ Hc : Comp _ (EPrimOp _) |- _ ] => inversion Hc
+  | [ Hc : Comp _ (EBot _) |- _ ] => inversion Hc
+  | [ Hc : Comp _ (EThunk _ (ELam _ _)) |- _ ] => inversion Hc; discriminate
+  | [ Hl : lookup_env _ _ = None, Hs : lookup_env _ _ = Some _ |- _ ] => congruence
+  end.
+
+Lemma read_shape : forall i Γ Φ k v,
+  resolves i Γ -> eval (Fin k) Φ Γ (EVar gv) v ->
+  (v = EBot BOutOfFuel /\ k <= S i) \/ (exists Γ0, v = EThunk Γ0 junk_fun).
+Proof.
+  intros i Γ Φ k v HR. revert Φ k v.
+  induction HR as [Γ Γ0 Hl | i Γ Γ0 Hl HR IH]; intros Φ k v H;
+    (destruct k as [| k]; [left; split; [exact (eval_fin_zero_inv _ _ _ _ H) | lia] |]);
+    inversion H; subst; try kill_rule;
+    match goal with
+    | [ Hs : lookup_env _ _ = Some _, Hv : eval (dec _) _ _ _ _ |- _ ] =>
+        rewrite Hl in Hs; injection Hs as <- <-; rewrite dec_remaining in Hv
+    end.
+  - destruct k as [| k]; [left; split; [exact (eval_fin_zero_inv _ _ _ _ H5) | lia] |].
+    unfold junk_fun in H5. inversion H5; subst; try kill_rule.
+    right. eexists. reflexivity.
+  - destruct (IH _ _ _ H5) as [[-> Hk] | Hr]; [left; split; [reflexivity | lia] | right; exact Hr].
+Qed.
+
+Lemma read_total : forall i Γ Φ k,
+  resolves i Γ ->
+  exists v, eval (Fin k) Φ Γ (EVar gv) v
+    /\ (v = EBot BOutOfFuel \/ exists Γ0, v = EThunk Γ0 junk_fun).
+Proof.
+  intros i Γ Φ k HR. revert Φ k.
+  induction HR as [Γ Γ0 Hl | i Γ Γ0 Hl HR IH]; intros Φ k;
+    (destruct k as [| k]; [exists (EBot BOutOfFuel); split; [apply Eval_OutOfFuel | left; reflexivity] |]).
+  - destruct k as [| k].
+    + exists (EBot BOutOfFuel). split; [eapply Eval_Var; [exact Hl | apply Eval_OutOfFuel] | left; reflexivity].
+    + exists (EThunk Γ0 junk_fun). split; [eapply Eval_Var; [exact Hl | apply Eval_Lam] | right; eexists; reflexivity].
+  - destruct (IH Φ k) as [v [Hv Hs]]. exists v. split; [eapply Eval_Var; [exact Hl | exact Hv] | exact Hs].
+Qed.
+
+Lemma resolves_link : forall i Γ Γ0,
+  resolves i Γ -> resolves (S i) (ExtendEnv gv (MkClosure Γ (EVar gv)) Γ0).
+Proof.
+  intros i Γ Γ0 HR. eapply Resolves_Link; [| exact HR]. reflexivity.
+Qed.
+
+Lemma resolves_fun : forall Γ Γ0,
+  resolves 0 (ExtendEnv gv (MkClosure Γ junk_fun) Γ0).
+Proof. intros Γ Γ0. eapply Resolves_Fun. reflexivity. Qed.
+
+Lemma resolves_bound : forall i Γ, resolves i Γ -> lookup_env Γ gv <> None.
+Proof. intros i Γ HR. destruct HR; congruence. Qed.
+
+Lemma app_bot_value : forall Φ Γ k ea v,
+  eval (Fin k) Φ Γ (EApp (EBot BOutOfFuel) ea) v -> v = EBot BOutOfFuel.
+Proof.
+  intros Φ Γ k ea v H. destruct k as [| k]; [exact (eval_fin_zero_inv _ _ _ _ H) |].
+  inversion H; subst; try kill_rule; reflexivity.
+Qed.
+
+Lemma junk_bound : forall k,
+  (forall i Γ Φ v, resolves i Γ -> eval (Fin k) Φ Γ junk_body v ->
+     tower v /\ k <= 4 * nots v + i) /\
+  (forall i Γ Φ v, resolves i Γ -> eval (Fin k) Φ Γ junk_arg v ->
+     tower v /\ k <= 4 * nots v + i + 3).
+Proof.
+  intros k. induction k as [k IH] using lt_wf_ind.
+  destruct k as [| k].
+  { split; intros i Γ Φ v _ H; apply eval_fin_zero_inv in H; subst; split; [constructor | lia | constructor | lia]. }
+  split; intros i Γ Φ v HR H.
+  - unfold junk_body in H. inversion H; subst; try kill_rule.
+    simpl in H3. injection H3 as <- <-.
+    inversion H8 as [| a w rest rest' Hw Hrest]; subst.
+    inversion Hrest; subst.
+    rewrite dec_remaining in Hw.
+    destruct (proj2 (IH k (Nat.lt_succ_diag_r k)) i Γ Φ w HR Hw) as [Ht Hk].
+    rewrite (reduce_not_tower w Ht). simpl nots. split; [constructor; exact Ht | lia].
+  - unfold junk_arg in H. inversion H; subst; try kill_rule.
+    match goal with
+    | [ Hf : eval _ _ _ (EVar gv) ?w, Ha : eval _ _ _ (EApp ?w (EVar gv)) _ |- _ ] =>
+        rewrite dec_remaining in Hf, Ha;
+        destruct (read_shape i Γ Φ k w HR Hf) as [[-> Hk] | [Γ0 ->]]
+    end.
+    + match goal with [Ha : eval _ _ _ (EApp (EBot _) _) _ |- _] => rewrite (app_bot_value _ _ _ _ _ Ha) end.
+      split; [constructor | simpl; lia].
+    + destruct k as [| k].
+      * match goal with [Ha : eval (Fin 0) _ _ (EApp _ _) _ |- _] => apply eval_fin_zero_inv in Ha end.
+        subst. split; [constructor | simpl; lia].
+      * match goal with [Ha : eval _ _ _ (EApp (EThunk _ _) _) _ |- _] =>
+          unfold junk_fun in Ha; inversion Ha; subst; try kill_rule end.
+        match goal with [Hb : eval _ _ _ junk_body _ |- _] =>
+          rewrite dec_remaining in Hb;
+          destruct (proj1 (IH k ltac:(lia)) (S i) _ Φ v (resolves_link i Γ Γ0 HR) Hb) as [Ht Hk]
+        end.
+        split; [exact Ht | lia].
+Qed.
+
+Lemma junk_value_bound : forall Γ Φ k v,
+  eval (Fin k) Φ Γ junk v -> tower v /\ k <= 4 * nots v + 2.
+Proof.
+  intros Γ Φ k v H. destruct k as [| k].
+  { apply eval_fin_zero_inv in H. subst. split; [constructor | lia]. }
+  unfold junk in H. inversion H; subst; try kill_rule.
+  match goal with
+  | [ Hf : eval _ _ _ junk_fun ?w, Ha : eval _ _ _ (EApp ?w junk_fun) _ |- _ ] =>
+      rewrite dec_remaining in Hf, Ha; destruct k as [| k]
+  end.
+  - match goal with [Hf : eval (Fin 0) _ _ junk_fun _ |- _] => apply eval_fin_zero_inv in Hf end.
+    subst. match goal with [Ha : eval _ _ _ (EApp (EBot _) _) _ |- _] => rewrite (app_bot_value _ _ _ _ _ Ha) end.
+    split; [constructor | simpl; lia].
+  - match goal with [Hf : eval _ _ _ junk_fun _ |- _] => unfold junk_fun in Hf; inversion Hf; subst; try kill_rule end.
+    match goal with [Ha : eval _ _ _ (EApp (EThunk _ _) _) _ |- _] => inversion Ha; subst; try kill_rule end.
+    match goal with [Hb : eval _ _ _ junk_body _ |- _] =>
+      rewrite dec_remaining in Hb;
+      destruct (proj1 (junk_bound k) 0 _ Φ v (resolves_fun Γ Γ) Hb) as [Ht Hk]
+    end.
+    split; [exact Ht | lia].
+Qed.
+
+Lemma junk_total : forall k,
+  (forall i Γ Φ, resolves i Γ -> exists v, eval (Fin k) Φ Γ junk_body v) /\
+  (forall i Γ Φ, resolves i Γ -> exists v, eval (Fin k) Φ Γ junk_arg v).
+Proof.
+  intros k. induction k as [k IH] using lt_wf_ind.
+  destruct k as [| k].
+  { split; intros; exists (EBot BOutOfFuel); apply Eval_OutOfFuel. }
+  split; intros i Γ Φ HR.
+  - destruct (proj2 (IH k (Nat.lt_succ_diag_r k)) i Γ Φ HR) as [w Hw].
+    eexists. unfold junk_body. eapply Eval_AppPrim; [reflexivity | reflexivity |].
+    constructor; [exact Hw | constructor].
+  - destruct (read_total i Γ Φ k HR) as [w [Hw [-> | [Γ0 ->]]]].
+    + exists (EBot BOutOfFuel). unfold junk_arg.
+      eapply Eval_AppSpine; [apply Comp_Var; exact (resolves_bound i Γ HR) | exact Hw |].
+      destruct k; [apply Eval_OutOfFuel | apply Eval_AppBot].
+    + destruct k as [| k].
+      * exists (EBot BOutOfFuel). unfold junk_arg.
+        eapply Eval_AppSpine; [apply Comp_Var; exact (resolves_bound i Γ HR) | exact Hw | apply Eval_OutOfFuel].
+      * destruct (proj1 (IH k ltac:(lia)) (S i) (ExtendEnv gv (MkClosure Γ (EVar gv)) Γ0) Φ
+                    (resolves_link i Γ Γ0 HR)) as [v Hv].
+        exists v. unfold junk_arg.
+        eapply Eval_AppSpine; [apply Comp_Var; exact (resolves_bound i Γ HR) | exact Hw |].
+        unfold junk_fun. apply Eval_AppAbs. exact Hv.
+Qed.
+
+Lemma junk_has_value : forall Γ Φ k, exists v, eval (Fin k) Φ Γ junk v.
+Proof.
+  intros Γ Φ k. destruct k as [| [| k]].
+  - exists (EBot BOutOfFuel). apply Eval_OutOfFuel.
+  - exists (EBot BOutOfFuel). unfold junk.
+    eapply Eval_AppSpine; [apply Comp_Lam | apply Eval_OutOfFuel | apply Eval_OutOfFuel].
+  - destruct (proj1 (junk_total k) 0 (ExtendEnv gv (MkClosure Γ junk_fun) Γ) Φ (resolves_fun Γ Γ))
+      as [v Hv].
+    exists v. unfold junk.
+    eapply Eval_AppSpine; [apply Comp_Lam | unfold junk_fun; apply Eval_Lam |].
+    unfold junk_fun. apply Eval_AppAbs. exact Hv.
 Qed.
